Prove SoundSnapshot except unary

coq/proof/SoundSnapshot.v
@@ -28,10 +28,20 @@ Set Implicit Arguments.
 
 (* TODO: lemma on tag.previous *)
 
+(* TODO: Unify this snapshot_specs *)
+
 Definition snapshot_as_previous st invst: Prop :=
   forall x gvx
-         (LOCAL_IN: lookupAL _ st.(EC).(Locals) x = Some gvx),
+         (LOCAL: lookupAL _ st.(EC).(Locals) x = Some gvx),
     <<PREV: InvState.Unary.sem_idT st invst (Tag.previous, x) = Some gvx>>.
+
+Definition snapshot_spec2 st invst: Prop :=
+  forall x gvx
+         (PREV: InvState.Unary.sem_idT st invst (Tag.previous, x) = Some gvx),
+    <<LOCAL: lookupAL _ st.(EC).(Locals) x = Some gvx>>.
+
+Definition snapshot_spec3 invst0 invst1: Prop :=
+  invst0.(InvState.Unary.ghost) = invst1.(InvState.Unary.ghost).
 
 Lemma snapshot_unary_sound
       conf st invst0 invmem inv0
@@ -39,9 +49,243 @@ Lemma snapshot_unary_sound
   :
     exists invst1,
       <<STATE: InvState.Unary.sem conf st invst1 invmem (Snapshot.unary inv0)>> /\
-               <<PREV: snapshot_as_previous st invst1>>.
+               <<PREV: snapshot_as_previous st invst1>> /\
+                       <<PREV2: snapshot_spec2 st invst1>> /\
+                                <<GHOST: snapshot_spec3 invst0 invst1>>.
+Proof.
+  exists (InvState.Unary.mk st.(EC).(Locals) invst0.(InvState.Unary.ghost)).
+  splits; ss.
+  inv STATE.
+  econs; ss.
+  - ii.
+    exploit ExprPairSet.union_1; eauto. i. des.
+    + admit.
+      (* Lemma snapshot_physical_previous_lessdef_spec *)
+      (*       Snapshot.unary *)
+    + admit.
+  - admit.
+  - admit.
+  - admit.
+  (* { clear -NOALIAS. inv NOALIAS. *)
+  (*   econs. *)
+  (*   - i. *)
+
+  
+  (* -  *)
+  (* Check (dom st.(EC).(Locals)). *)
+
+  (* esplits. *)
+Admitted.
+
+Lemma IdTSet_map_aux
+      f tx (elems:list IdT.t)
+  :
+      <<REV: IdTSet.In tx (fold_right (IdTSet.add <*> f) IdTSet.empty (rev elems))
+                          <-> IdTSet.In tx (fold_right (IdTSet.add <*> f) IdTSet.empty elems)>>.
 Proof.
 Admitted.
+
+Lemma IdTSet_map_spec
+      f s ty
+      (IN: IdTSet.In ty (IdTSet_map f s))
+  :
+    exists tx, <<IN: IdTSet.In tx s>> /\
+                    <<MAP: f tx = ty>>.
+Proof.
+  unfold IdTSet_map in *.
+  rewrite IdTSet.fold_1 in *.
+  remember (IdTSet.elements s) as elems.
+  assert (INEQ: forall x, In x elems <-> In x (IdTSet.elements s)).
+  { subst. eauto. }
+  assert (NODUP: NoDup elems).
+  { subst. apply push_iter.NoDupA__NoDup.
+    apply IdTSet.elements_3w. }
+  clear Heqelems.
+  rewrite <- fold_left_rev_right in IN.
+  assert (REV: forall ty, IdTSet.In ty (fold_right (IdTSet.add <*> f) IdTSet.empty (rev elems))
+                          <-> IdTSet.In ty (fold_right (IdTSet.add <*> f) IdTSet.empty elems)).
+  { i. apply IdTSet_map_aux. }
+  rewrite REV in IN. clear REV.
+  revert s ty IN INEQ NODUP.
+  induction elems.
+  { i. ss. exfalso. eapply IdTSetFacts.empty_iff; eauto. }
+  i. ss.
+  apply IdTSetFacts.add_iff in IN. des.
+  { esplits; eauto.
+    apply IdTSet.elements_2.
+    specialize (INEQ a). des.
+    exploit INEQ; eauto.
+    i. apply InA_iff_In; eauto.
+  }
+  { specialize (IHelems (IdTSet.remove a s)).
+    inv NODUP.
+    exploit IHelems; eauto.
+    { split.
+      - i.
+        specialize (INEQ x). des.
+        exploit INEQ; eauto. i.
+        rewrite <- InA_iff_In in *.
+        apply IdTSetFacts.elements_iff.
+        apply IdTSetFacts.remove_iff.
+        split.
+        + apply IdTSetFacts.elements_iff. eauto.
+        + ii. subst. eauto.
+      - i.
+        rewrite <- InA_iff_In in H.
+        apply IdTSetFacts.elements_iff in H.
+        apply IdTSetFacts.remove_iff in H. des.
+        apply IdTSet.elements_1 in H.
+        rewrite InA_iff_In in H.
+        apply INEQ in H. des; done.
+    }
+    i. des.
+    esplits; eauto.
+    eapply IdTSet.remove_3; eauto.
+  }
+Qed.
+
+Lemma IdTSet_map_spec2
+      f s tx
+      (IN: IdTSet.In tx s)
+  :
+    <<IN: IdTSet.In (f tx) (IdTSet_map f s)>>.
+Proof.
+  unfold IdTSet_map.
+  rewrite IdTSet.fold_1.
+  rewrite <- fold_left_rev_right.
+  apply IdTSet_map_aux.
+  remember (IdTSet.elements s) as elems.
+  assert (INEQ: forall x, In x elems <-> In x (IdTSet.elements s)).
+  { subst. eauto. }
+  assert (NODUP: NoDup elems).
+  { subst. apply push_iter.NoDupA__NoDup.
+    apply IdTSet.elements_3w. }
+  clear Heqelems.
+  
+  revert s tx IN INEQ NODUP.
+  induction elems.
+  - i. ss.
+    apply IdTSet.elements_1 in IN.
+    apply InA_iff_In in IN.
+    exfalso. eapply INEQ. eauto.
+  - i. ss.
+    specialize (IHelems (IdTSet.remove a s)).
+    inv NODUP.
+    apply IdTSetFacts.add_iff.
+    destruct (IdT.eq_dec a tx).
+    { subst. eauto. }
+    right.
+    exploit IHelems; eauto.
+    + apply IdTSetFacts.remove_iff; eauto.
+    + split.
+      { i.
+        rewrite <- InA_iff_In.
+        apply IdTSetFacts.elements_iff.
+        apply IdTSetFacts.remove_iff.
+        split.
+        - apply IdTSetFacts.elements_iff.
+          rewrite InA_iff_In.
+          apply INEQ; eauto.
+        - ii. subst. done.
+      }
+      { i.
+        rewrite <- InA_iff_In in H.
+        apply IdTSetFacts.elements_iff in H.
+        apply IdTSetFacts.remove_iff in H. des.
+        apply IdTSetFacts.elements_iff in H.
+        rewrite InA_iff_In in H.
+        apply INEQ in H. des; done.
+      }
+Qed.
+
+Lemma snapshot_maydiff_spec1
+      md0 x t
+      (IN: IdTSet.In (t, x) md0)
+      (NOTPREV: t <> Tag.previous)
+  :
+    <<IN: IdTSet.In (t, x) (Snapshot.IdTSet md0)>>.
+Proof.
+  unfold Snapshot.IdTSet.
+  apply IdTSet.union_2.
+  apply IdTSet.filter_3; eauto.
+  { ii. subst. ss. }
+  destruct t; eauto.
+Qed.
+
+Lemma snapshot_maydiff_spec1_inv
+      md0 x t
+      (NOTIN: ~ IdTSet.mem (t, x) (Snapshot.IdTSet md0))
+      (NOTPREV: t <> Tag.previous)
+  :
+    <<NOTIN: ~ IdTSet.mem (t, x) md0>>.
+Proof.
+  destruct (IdTSet.mem (t, x) md0) eqn:MEM; eauto.
+  apply IdTSet.mem_2 in MEM.
+  apply snapshot_maydiff_spec1 in MEM; eauto.
+  des. apply IdTSet.mem_1 in MEM. done.
+Qed.
+
+Lemma snapshot_maydiff_spec2
+      md0 x
+      (IN: IdTSet.In (Tag.previous, x) (Snapshot.IdTSet md0))
+  :
+    <<IN: IdTSet.In (Tag.physical, x) md0 >>.
+Proof.
+  unfold Snapshot.IdTSet in IN.
+  apply IdTSet.union_1 in IN. des.
+  { apply IdTSetFacts.filter_iff in IN; cycle 1.
+    { ii. subst. ss. }
+    des. ss.
+  }
+  apply IdTSet_map_spec in IN. des.
+  apply IdTSetFacts.filter_iff in IN0; cycle 1.
+  { ii. subst. ss. }
+  des.
+  unfold compose in *.
+  unfold Previousify.IdT in *.
+  destruct tx.
+  destruct t; ss.
+  inv MAP; eauto.
+Qed.
+
+Lemma snapshot_maydiff_spec2_inv
+      md0 x
+      (NOTIN: ~ IdTSet.mem (Tag.physical, x) md0)
+  :
+    <<NOTIN: ~ IdTSet.mem (Tag.previous, x) (Snapshot.IdTSet md0) >>.
+Proof.
+  destruct (IdTSet.mem (Tag.previous, x) (Snapshot.IdTSet md0)) eqn:MEM; eauto.
+  apply IdTSet.mem_2 in MEM.
+  apply snapshot_maydiff_spec2 in MEM; try done.
+  des. apply IdTSet.mem_1 in MEM. done.
+Qed.
+
+Lemma snapshot_maydiff_spec3
+      md0 x
+      (IN: IdTSet.In (Tag.physical, x) md0)
+  :
+    <<IN: IdTSet.In (Tag.previous, x) (Snapshot.IdTSet md0)>>.
+Proof.
+  unfold Snapshot.IdTSet.
+  apply IdTSet.union_3.
+  replace (Tag.previous, x) with (Previousify.IdT (Tag.physical, x)); eauto.
+  apply IdTSet_map_spec2.
+  apply IdTSetFacts.filter_iff.
+  { ii. subst. ss. }
+  split; eauto.
+Qed.
+
+Lemma snapshot_maydiff_spec3_inv
+      md0 x
+      (IN: ~ IdTSet.mem (Tag.previous, x) (Snapshot.IdTSet md0))
+  :
+    <<IN: ~ IdTSet.mem (Tag.physical, x) md0>>.
+Proof.
+  destruct (IdTSet.mem (Tag.physical, x) md0) eqn:MEM; eauto.
+  apply IdTSet.mem_2 in MEM.
+  apply snapshot_maydiff_spec3 in MEM; try done.
+  des. apply IdTSet.mem_1 in MEM. done.
+Qed.
 
 Lemma snapshot_sound
       conf_src conf_tgt st_src st_tgt invst0 invmem inv0
@@ -52,22 +296,37 @@ Lemma snapshot_sound
     <<PREV_TGT: snapshot_as_previous st_tgt invst1.(InvState.Rel.tgt)>>.
 Proof.
   inv STATE.
-  apply snapshot_unary_sound in SRC.
+  apply snapshot_unary_sound in SRC. des.
   apply snapshot_unary_sound in TGT. des.
+  exists (InvState.Rel.mk invst1 invst2).
   esplits.
   - econs.
-    + admit.
-    + admit.
-    + admit.
-      (* Lemma snapshot_maydiff_incr *)
-      (*       Snapshot.IdTSet maydiff *)
-
-
-
-    
-  
-
-
-
-  
-Admitted.
+    + ss.
+    + ss.
+    + ss.
+      i.
+      destruct id0.
+      destruct t.
+      { hexploit snapshot_maydiff_spec1_inv; eauto; try done. i. des.
+        hexploit MAYDIFF; eauto.
+      }
+      { hexploit snapshot_maydiff_spec3_inv; eauto. i. des.
+        hexploit MAYDIFF; eauto. i.
+        ii. ss.
+        exploit PREV2; eauto. i. des.
+        exploit H0.
+        { unfold InvState.Unary.sem_idT. ss. eauto. }
+        i. des.
+        esplits; eauto.
+        exploit PREV0; eauto.
+      }
+      { hexploit snapshot_maydiff_spec1_inv; eauto; try done. i. des.
+        hexploit MAYDIFF; eauto. i.
+        unfold snapshot_spec3 in *.
+        unfold InvState.Rel.sem_inject in *.
+        unfold InvState.Unary.sem_idT in *. ss.
+        rewrite <- GHOST. rewrite <- GHOST0. eauto.
+      }
+  - eauto.
+  - eauto.
+Qed.
